src/RqRsFacts.v
@@ -183,7 +183,7 @@ Section RqRsDTree.
           parentIdxOf dtr cidx = Some oidx /\
           edgeDownTo dtr cidx = Some down /\
           rsEdgeUpFrom dtr cidx = Some rsUp /\
-          In rsUp rssFrom.
+          In rsUp (map fst rssFrom).
   Proof.
     intros.
     red in H; dest; clear H.
@@ -204,7 +204,7 @@ Section RqRsDTree.
     forall oidx rssFrom rqTos P,
       RqRsDownMatch dtr oidx rqTos rssFrom P ->
       forall rsUp,
-        In rsUp rssFrom ->
+        In rsUp (map fst rssFrom) ->
         exists cidx down,
           P cidx /\
           parentIdxOf dtr cidx = Some oidx /\
@@ -447,7 +447,7 @@ Section RqRsDTree.
     forall oidx1 oidx2 rqUp1 downs2 ups2 P,
       rqEdgeUpFrom dtr oidx1 = Some rqUp1 ->
       RqRsDownMatch dtr oidx2 downs2 ups2 P ->
-      ~ In rqUp1 ups2.
+      ~ In rqUp1 (map fst ups2).
   Proof.
     intros; intro Hx.
     eapply RqRsDownMatch_rs_rq in H0; [|eassumption].
@@ -459,7 +459,7 @@ Section RqRsDTree.
     forall oidx rsUp1 downs2 ups2 P,
       rsEdgeUpFrom dtr oidx = Some rsUp1 ->
       RqRsDownMatch dtr oidx downs2 ups2 P ->
-      ~ In rsUp1 ups2.
+      ~ In rsUp1 (map fst ups2).
   Proof.
     intros; intro Hx.
     eapply RqRsDownMatch_rs_rq in H0; [|eassumption].
@@ -473,7 +473,7 @@ Section RqRsDTree.
       rsEdgeUpFrom dtr oidx1 = Some rsUp1 ->
       RqRsDownMatch dtr oidx2 downs2 ups2 P ->
       parentIdxOf dtr oidx1 <> Some oidx2 ->
-      ~ In rsUp1 ups2.
+      ~ In rsUp1 (map fst ups2).
   Proof.
     intros; intro Hx.
     eapply RqRsDownMatch_rs_rq in H0; [|eassumption].
@@ -487,7 +487,7 @@ Section RqRsDTree.
     forall oidx1 oidx2 down1 downs2 ups2 P,
       edgeDownTo dtr oidx1 = Some down1 ->
       RqRsDownMatch dtr oidx2 downs2 ups2 P ->
-      ~ In down1 ups2.
+      ~ In down1 (map fst ups2).
   Proof.
     intros; intro Hx.
     eapply RqRsDownMatch_rs_rq in H0; [|eassumption].
@@ -585,7 +585,7 @@ Section RqRsDTree.
       oidx1 <> oidx2 ->
       RqRsDownMatch dtr oidx1 rqTos1 rssFrom1 P1 ->
       RqRsDownMatch dtr oidx2 rqTos2 rssFrom2 P2 ->
-      DisjList rssFrom1 rssFrom2.
+      DisjList (map fst rssFrom1) (map fst rssFrom2).
   Proof.
     intros.
     apply (DisjList_false_spec idx_dec); intros midx ? ?.
@@ -603,7 +603,7 @@ Section RqRsDTree.
       parentIdxOf dtr cidx = Some oidx ->
       edgeDownTo dtr cidx = Some down ->
       rsEdgeUpFrom dtr cidx = Some rsUp ->
-      ~ In rsUp ups ->
+      ~ In rsUp (map fst ups) ->
       RqRsDownMatch dtr oidx downs ups P ->
       ~ In down downs.
   Proof.
@@ -647,7 +647,7 @@ Section RqRsDTree.
     forall oidx rqTos rssFrom1 rssFrom2 P1 P2,
       RqRsDownMatch dtr oidx rqTos rssFrom1 P1 ->
       RqRsDownMatch dtr oidx rqTos rssFrom2 P2 ->
-      rssFrom1 = rssFrom2.
+      map fst rssFrom1 = map fst rssFrom2.
   Proof.
     unfold RqRsDownMatch; intros; dest.
     clear H H0.
@@ -694,7 +694,7 @@ Section RqRsDTree.
            rrFrom1 rrFrom2 rssFrom1 rssFrom2,
       FootprintUpDownOk dtr sys oidx rrFrom1 rqTos rssFrom1 ->
       FootprintUpDownOk dtr sys oidx rrFrom2 rqTos rssFrom2 ->
-      rssFrom1 = rssFrom2.
+      map fst rssFrom1 = map fst rssFrom2.
   Proof.
     unfold FootprintUpDownOk; intros.
     destruct rrFrom1 as [[rqFrom1 rsbTo1]|], rrFrom2 as [[rqFrom2 rsbTo2]|].
@@ -720,7 +720,7 @@ Section RqRsDTree.
     forall oidx rqFrom rqTos rssFrom1 rsbTo1 rssFrom2 rsbTo2,
       FootprintDownDownOk dtr oidx rqFrom rqTos rssFrom1 rsbTo1 ->
       FootprintDownDownOk dtr oidx rqFrom rqTos rssFrom2 rsbTo2 ->
-      rssFrom1 = rssFrom2 /\ rsbTo1 = rsbTo2.
+      map fst rssFrom1 = map fst rssFrom2 /\ rsbTo1 = rsbTo2.
   Proof.
     unfold FootprintDownDownOk; intros.
     dest; split.
@@ -1056,6 +1056,7 @@ Ltac disc_rule_conds_unit_simpl :=
     destruct rins as [|[rin rmsg] [|]]; try discriminate;
     simpl in H; inv H
   | [H: idsOf [_] = [_]%list |- _] => simpl in H; inv H
+  | [H: idsOf _ = map fst _ |- _] => rewrite H in *
 
   | [H: _ :: nil = _ :: nil |- _] => inv H
   | [H: nil = nil |- _] => clear H
@@ -1069,7 +1070,7 @@ Ltac disc_rule_conds_unit_simpl :=
   | [H1: msg_type ?msg = MRq, H2: msg_type ?msg = MRs |- _] =>
     rewrite H1 in H2; discriminate
   | [H: rqi_msg _ = _ |- _] => rewrite H in *
-  | [H: rqi_minds_rss _ = _ |- _] => rewrite H in *
+  | [H: rqi_rss _ = _ |- _] => rewrite H in *
   | [H: rqi_midx_rsb _ = _ |- _] => rewrite H in *
   end.
 
@@ -1534,19 +1535,19 @@ Ltac solve_midx_neq_unit :=
     eapply rqrsDTree_down_downs_not_in; eauto
 
   | [Hru1: rqEdgeUpFrom _ ?idx1 = Some ?rqUp1,
-     Hdowns2: RqRsDownMatch _ ?idx2 _ ?ups2 _ |- ~ In ?rqUp1 ?ups2] =>
+     Hdowns2: RqRsDownMatch _ ?idx2 _ ?ups2 _ |- ~ In ?rqUp1 (map fst ?ups2)] =>
     eapply rqrsDTree_rqUp_ups_not_in; eauto
   | [Hru1: rsEdgeUpFrom _ ?idx = Some ?rsUp1,
-     Hdowns2: RqRsDownMatch _ ?idx _ ?ups2 _ |- ~ In ?rsUp1 ?ups2] =>
+     Hdowns2: RqRsDownMatch _ ?idx _ ?ups2 _ |- ~ In ?rsUp1 (map fst ?ups2)] =>
     eapply rqrsDTree_rsUp_ups_not_in; eauto
   | [Hdown1: edgeDownTo _ ?idx1 = Some ?down1,
-     Hdowns2: RqRsDownMatch _ ?idx2 _ ?ups2 _ |- ~ In ?down1 ?ups2] =>
+     Hdowns2: RqRsDownMatch _ ?idx2 _ ?ups2 _ |- ~ In ?down1 (map fst ?ups2)] =>
     eapply rqrsDTree_down_ups_not_in; eauto
 
   | [Hru1: rsEdgeUpFrom _ ?idx1 = Some ?rsUp1,
      Hdowns2: RqRsDownMatch _ ?idx2 _ ?ups2 _,
      Hp: parentIdxOf _ ?idx1 = Some ?pidx,
-     Hnp: Some ?pidx <> Some ?idx2 |- ~ In ?rqUp1 ?ups2] =>
+     Hnp: Some ?pidx <> Some ?idx2 |- ~ In ?rqUp1 (map fst ?ups2)] =>
     rewrite <-Hp in Hnp;
     eapply rqrsDTree_rsUp_ups_not_in_parent; eauto
   | [Hdown1: edgeDownTo _ ?idx1 = Some ?down1,
@@ -1563,7 +1564,7 @@ Ltac solve_midx_neq_unit :=
   | [Hp: parentIdxOf _ ?cidx = Some ?oidx,
      Hdown: edgeDownTo _ ?cidx = Some ?down,
      Hup: rsEdgeUpFrom _ ?cidx = Some ?rsUp,
-     Hnin: ~ In ?rsUp ?ups,
+     Hnin: ~ In ?rsUp (map fst ?ups),
      Hud: RqRsDownMatch _ ?oidx ?downs ?ups _ |- ~ In ?down ?downs] =>
     eapply rqrsDTree_down_downs_not_in_child; eauto
   end.
